soundness: regenerate F* models

securedrop-protocol/protocol-minimal/proofs/fstar/models/Libcrux_ml_kem.Types.fsti
@@ -6,6 +6,15 @@ open Core_models
 ///An ML-KEM Ciphertext
 type t_MlKemCiphertext (v_SIZE: usize) = { f_value:t_Array u8 v_SIZE }
 
+/// A reference to the raw byte slice.
+val impl_7__as_slice (v_SIZE: usize) (self: t_MlKemCiphertext v_SIZE)
+    : Prims.Pure (t_Array u8 v_SIZE)
+      Prims.l_True
+      (ensures
+        fun result ->
+          let result:t_Array u8 v_SIZE = result in
+          result == self.f_value)
+
 ///An ML-KEM Private key
 type t_MlKemPrivateKey (v_SIZE: usize) = { f_value:t_Array u8 v_SIZE }
 
@@ -13,12 +22,30 @@ type t_MlKemPrivateKey (v_SIZE: usize) = { f_value:t_Array u8 v_SIZE }
 val impl_14 (v_SIZE: usize)
     : Core_models.Convert.t_From (t_MlKemPrivateKey v_SIZE) (t_Array u8 v_SIZE)
 
+/// A reference to the raw byte slice.
+val impl_15__as_slice (v_SIZE: usize) (self: t_MlKemPrivateKey v_SIZE)
+    : Prims.Pure (t_Array u8 v_SIZE)
+      Prims.l_True
+      (ensures
+        fun result ->
+          let result:t_Array u8 v_SIZE = result in
+          result == self.f_value)
+
 ///An ML-KEM Public key
 type t_MlKemPublicKey (v_SIZE: usize) = { f_value:t_Array u8 v_SIZE }
 
 [@@ FStar.Tactics.Typeclasses.tcinstance]
 val impl_22 (v_SIZE: usize)
     : Core_models.Convert.t_From (t_MlKemPublicKey v_SIZE) (t_Array u8 v_SIZE)
+
+/// A reference to the raw byte slice.
+val impl_23__as_slice (v_SIZE: usize) (self: t_MlKemPublicKey v_SIZE)
+    : Prims.Pure (t_Array u8 v_SIZE)
+      Prims.l_True
+      (ensures
+        fun result ->
+          let result:t_Array u8 v_SIZE = result in
+          result == self.f_value)
 
 /// An ML-KEM key pair
 type t_MlKemKeyPair (v_PRIVATE_KEY_SIZE: usize) (v_PUBLIC_KEY_SIZE: usize) = {
