securedrop-protocol/protocol-minimal/proofs/fstar/extraction/Securedrop_protocol_minimal.Primitives.Provider.Ed25519.fst
@@ -1,0 +1,40 @@
+module Securedrop_protocol_minimal.Primitives.Provider.Ed25519
+#set-options "--fuel 0 --ifuel 1 --z3rlimit 15"
+open FStar.Mul
+open Core_models
+
+let _ =
+  (* This module has implicit dependencies, here we make them explicit. *)
+  (* The implicit dependencies arise from typeclasses instances. *)
+  let open Rand_core in
+  ()
+
+/// Generate an ed25519 keypair
+assume
+val keygen': #v_R: Type0 -> {| i0: Rand_core.t_CryptoRng v_R |} -> rng: v_R
+  -> (v_R &
+      Core_models.Result.t_Result (t_Array u8 (mk_usize 32) & t_Array u8 (mk_usize 32))
+        Anyhow.t_Error)
+
+unfold
+let keygen (#v_R: Type0) (#[FStar.Tactics.Typeclasses.tcresolve ()] i0: Rand_core.t_CryptoRng v_R) =
+  keygen' #v_R #i0
+
+/// Sign `payload` with Ed25519 secret key bytes.
+assume
+val sign': payload: t_Slice u8 -> private_key: t_Array u8 (mk_usize 32)
+  -> Core_models.Result.t_Result (t_Array u8 (mk_usize 64)) Anyhow.t_Error
+
+unfold
+let sign = sign'
+
+/// Verify an Ed25519 `signature` over `payload` with verifying key bytes.
+assume
+val verify':
+    payload: t_Slice u8 ->
+    public_key: t_Array u8 (mk_usize 32) ->
+    signature: t_Array u8 (mk_usize 64)
+  -> Core_models.Result.t_Result Prims.unit Anyhow.t_Error
+
+unfold
+let verify = verify'
